---
title: "연습장"
date: 2025-01-02 21:18:03 +0900
categories: [블로그, Github]
tags: [github]
use_math: true
published: false
---

연습장

$\begin{aligned}
y_i&=\beta_0+\beta_1x_i+\varepsilon_i\ (i=1, 2, \cdots, n)\\
\varepsilon_i&=y_i-\beta_0-\beta_1x_i\\
\sum^n_{i=1}\varepsilon_i^2&=\sum^n_{i=1}(y_i-\beta_0-\beta_1x_i)^2\\
S(\beta_0, \beta_1)&=\sum^n_{i=1}(y_i-\beta_0-\beta_1x_i)^2\\
\end{aligned}$  
We have to find $\beta_0, \beta_1$ minimize $S(\beta_0, \beta_1)$

$$\begin{cases}
\frac{\partial S}{\partial \beta_0}=0\\
\frac{\partial S}{\partial \beta_1}=0
\tag{2}
\end{cases}$$

$\begin{cases}
\hat{\beta_0}=\bar{y}-\hat{\beta}_1\bar{x}\\
\hat{\beta_1}=\frac{S_{XY}}{S_{XX}}=\frac{\sum^n_{i=1}(x_i-\bar{x})(y_i-\bar{y})}{\sum^n_{i=1}(x_i-\bar{x})^2}
\end{cases}$

$\begin{aligned}
S_{XY}&=\sum^n_{i=1}(x_i-\bar{x})(y_i-\bar{y})\\
&=\sum^n_{i=1}x_i(y_i-\bar{y})-\sum^n_{i=1}\bar{x}(y_i-\bar{y})\\
\because \sum^n_{i=1}(y_i-\bar{y})&=\sum^n_{i=1}y_i-\sum^n_{i=1}\bar{y}\\
&=\sum^n_{i=1}y_i-n\bar{y}\\
&=n(\frac{1}{n}\sum^n_{i=1}y_i-\bar{y})\\
\because \frac{1}{n}\sum^n_{i=1}y_i=\bar{y}\\
&=n(0-0)=0\\
\end{aligned}$

$\begin{aligned}
\therefore \sum^n_{i=1}x_i(y_i-\bar{y})-\sum^n_{i=1}\bar{x}(y_i-\bar{y})&=\sum^n_{i=1}x_i(y_i-\bar{y})
\end{aligned}$

> abcdefg

````python
a = int(input())
b = int(input())
def plus(a, b):
    result = a + b
    return result
print(plus(a, b))
````