---
title: "SST, SSR, SSE 관계 유도"
date: 2025-01-18 11:28:53 +0900
categories: [통계학, 회귀분석]
tags: [statistics, regression_analysis]
use_math: true
---

정의
$SST=\sum^n_{i=1}(y_i-\bar{y})^2 \tag{1}$  
$SSR=\sum^n_{i=1}(\hat{y}_i-\bar{y})^2 \tag{2}$  
$SSE=\sum^n_{i=1}(y_i-\hat{y}_i)^2 \tag{3}$  

### $SST=SSE+SSR$ 유도

$SST=\sum^n_{i=1}(y_i-\bar{y})^2 \tag{4}$  
$\sum^n_{i=1}(y_i-\bar{y})^2=\sum^n_{i=1}(y_i-\hat{y}_i+\hat{y}_i-\bar{y})^2 \tag{5}$
$\sum^n_{i=1}(y_i-\hat{y}_i+\hat{y}_i-\bar{y})^2=\sum^n_{i=1}[(y_i-\hat{y}_i)+(\hat{y}_i-\bar{y})]^2 \tag{6}$  
$\sum^n_{i=1}[(y_i-\hat{y}_i)+(\hat{y}_i-\bar{y})]^2=\sum^n_{i=1}[(y_i-\hat{y}_i)^2+2(y_i-\hat{y}_i)(\hat{y}_i-\bar{y})+(\hat{y}_i-\bar{y})^2] \tag{7}$  
$\sum^n_{i=1}[(y_i-\hat{y}_i)^2+2(y_i-\hat{y}_i)(\hat{y}_i-\bar{y})+(\hat{y}_i-\bar{y})^2]=\sum^n_{i=1}(y_i-\hat{y}_i)^2+\sum^n_{i=1}2(y_i-\hat{y}_i)(\hat{y}_i-\bar{y})+\sum^n_{i=1}(\hat{y}_i-\bar{y})^2 \tag{8}$  

(2), (3)을 (8)에 대입하면,
$\sum^n_{i=1}(y_i-\hat{y}_i)^2+\sum^n_{i=1}2(y_i-\hat{y}_i)(\hat{y}_i-\bar{y})+\sum^n_{i=1}(\hat{y}_i-\bar{y})^2=SSE+\sum^n_{i=1}2(y_i-\hat{y}_i)(\hat{y}_i-\bar{y})+SSR \tag{9}$  

$SST=SSE+SSR$이 되기 위해서는, $\sum^n_{i=1}2(y_i-\hat{y}_i)(\hat{y}_i-\bar{y})=0$가 성립해야 함.  
[최소제곱량 추정](https://jeongho0715.github.io/posts/2501180001/) (46)에 의해,
$\bar{y}=\hat{\beta}_ 0+\hat{\beta}_ 1\bar{x} \tag{10}$  

$\hat{y}_i=\hat{\beta}_0+\hat{\beta}_1x_i \tag{11}$  

$\sum^n_{i=1}(y_i-\hat{y}_i)(\hat{y}_i-\bar{y})\tag{12}$  
$\sum^n_{i=1}(y_i-\hat{y}_i)(\hat{y}_i-\bar{y})=\sum^n_{i=1}(y_i-\hat{\beta}_0+\hat{\beta}_1x_i)(\hat{\beta}_0+\hat{\beta}_1x_i-\hat{\beta}_ 0+\hat{\beta}_ 1\bar{x})\tag{13}$  
$\sum^n_{i=1}(y_i-\hat{\beta}_0+\hat{\beta}_1x_i)(\hat{\beta}_0+\hat{\beta}_1x_i-\hat{\beta}_ 0+\hat{\beta}_ 1\bar{x})=\sum^n_{i=1}(y_i-\hat{\beta}_0+\hat{\beta}_1x_i)(\hat{\beta}_1x_i+\hat{\beta}_ 1\bar{x}) \tag{13}$  
$\sum^n_{i=1}(y_i-\hat{\beta}_0+\hat{\beta}_1x_i)(\hat{\beta}_1x_i+\hat{\beta}_ 1\bar{x})=\hat{\beta}_1\sum^n_{i=1}(y_i-\hat{\beta}_0+\hat{\beta}_1x_i)(x_i+\bar{x}) \tag{13}$  
$\hat{\beta}_1\sum^n_{i=1}(y_i-\hat{\beta}_0+\hat{\beta}_1x_i)(x_i+\bar{x})=\hat{\beta}_1\sum^n_{i=1}y_i(x_i+\bar{x})-\hat{\beta}_0\hat{\beta}_1\sum^n_{i=1}(x_i+\bar{x})+\hat{\beta}_1^2\sum^n_{i=1}x_i(x_i+\bar{x}) \tag{14}$  
[최소제곱량 추정](https://jeongho0715.github.io/posts/2501180001/) (36)에 의해,
$\sum^n_{i=1}(x_i+\bar{x})=0 \tag{15}$  

(15)를 (14)에 대입하면,
$\hat{\beta}_1\sum^n_{i=1}y_i(x_i+\bar{x})-\hat{\beta}_0\hat{\beta}_1\sum^n_{i=1}(x_i+\bar{x})+\hat{\beta}_1^2\sum^n_{i=1}x_i(x_i+\bar{x})=\hat{\beta}_1\sum^n_{i=1}y_i(x_i+\bar{x})+\hat{\beta}_1^2\sum^n_{i=1}x_i(x_i+\bar{x}) \tag{16}$  

[최소제곱량 추정](https://jeongho0715.github.io/posts/2501180001/) (43)에 의해,
$\sum^n_{i=1}x_i(x_i+\bar{x})=\sum^n_{i=1}(x_i+\bar{x})^2 \tag{17}$  
$\sum^n_{i=1}y_i(x_i+\bar{x})=\sum^n_{i=1}(x_i+\bar{x})(y_i+\bar{y}) \tag{18}$  
(17), (18)을 (16)에 대입하면,

$\hat{\beta}_1\sum^n_{i=1}y_i(x_i+\bar{x})+\hat{\beta}_1^2\sum^n_{i=1}x_i(x_i+\bar{x})=\hat{\beta}_1\sum^n_{i=1}(x_i+\bar{x})(y_i+\bar{y})+\hat{\beta}_1^2\sum^n_{i=1}(x_i+\bar{x})^2 \tag{19}$  
$\hat{\beta}_1\sum^n_{i=1}(x_i+\bar{x})(y_i+\bar{y})+\hat{\beta}_1^2\sum^n_{i=1}(x_i+\bar{x})^2=\hat{\beta}_1 S_{XY}+\hat{\beta}_1^2S_{XX} \tag{20}$  
$\hat{\beta}_1 S_{XY}+\hat{\beta}_1^2S_{XX}=\hat{\beta}_1 (S_{XY}+\hat{\beta}_1S_{XX}) \tag{20}$  

[최소제곱량 추정](https://jeongho0715.github.io/posts/2501180001/) (47)에 의해,
$\hat{\beta}_1=\frac{S_{XY}}{S_{XX}} \tag{21}$

(21)을 (20)에 대입하면,
$\hat{\beta}_1(S_{XY}+\hat{\beta}_1S_{XX})=\hat{\beta}_1 (S_{XY}+\frac{S_{XY}}{S_{XX}}S_{XX}) \tag{22}$  
$\hat{\beta}_1(S_{XY}+\frac{S_{XY}}{S_{XX}}S_{XX})=\hat{\beta}_1(S_{XY}+S_{XY})=0 \tag{23}$  

(23)을 (9)에 대입하면,
$SSE+\sum^n_{i=1}2(y_i-\hat{y}_i)(\hat{y}_i-\bar{y})+SSR=SSE+SSR \tag{24}$  
따라서 $SST=SSE+SSR$ ■